added some eqb stuff but left TODOs

src/DatalogParams/ATLDatalogParams.v
@@ -1,10 +1,7 @@
 From Datalog Require Import Datalog.
-From DatalogRocq Require Import DependencyGenerator.
-From Stdlib Require Import List.
-From Stdlib Require Import String.
-From Stdlib Require Import Bool.Bool.
+From DatalogRocq Require Import DependencyGenerator EqbSpec.
+From Stdlib Require Import List String Bool ZArith.
 From Datalog Require Import ATLToDatalog.
-From Stdlib Require Import ZArith.Znat.
 Import ListNotations.
 Open Scope bool_scope.
 Open Scope string_scope.
@@ -20,9 +17,11 @@ Definition rule := Datalog.rule rel var fn aggregator.
 Definition program := list rule.
 Definition expr := Datalog.expr var fn.
 Definition fact := Datalog.fact rel var fn.
+Definition agg_expr := Datalog.agg_expr rel var fn aggregator.
 
 (* Equality *)
 Definition var_eqb : var -> var -> bool := ATLToDatalog.var_eqb.
+
 Definition var_eqb_spec : forall x y, BoolSpec (x = y) (x <> y) (var_eqb x y).
 Proof. apply ATLToDatalog.var_eqb_spec. Qed.
 
@@ -42,21 +41,10 @@ Proof.
 Qed.
 
 Definition rel_eqb (r1 r2 : rel) : bool :=
-    match r1, r2 with
-    | (rel1, b1), (rel2, b2) =>
-        ATLToDatalogRel_eqb rel1 rel2 && Bool.eqb b1 b2
-    end.
-
-Lemma pair_eqb_spec {A B} (eqbA : A -> A -> bool) (eqbB : B -> B -> bool)
-      (specA : forall x y, BoolSpec (x = y) (x <> y) (eqbA x y))
-      (specB : forall x y, BoolSpec (x = y) (x <> y) (eqbB x y))
-      (p1 p2 : A * B) :
-  BoolSpec (p1 = p2) (p1 <> p2)
-           (let (a1,b1) := p1 in let (a2,b2) := p2 in eqbA a1 a2 && eqbB b1 b2).
-Proof.
-  destruct p1 as [a1 b1], p2 as [a2 b2].
-  destruct (specA a1 a2); destruct (specB b1 b2); constructor; congruence.
-Qed.
+  match r1, r2 with
+  | (rel1, b1), (rel2, b2) =>
+      ATLToDatalogRel_eqb rel1 rel2 && Bool.eqb b1 b2
+  end.
 
 Definition rel_eqb_spec x y : BoolSpec (x = y) (x <> y) (rel_eqb x y).
 Proof.
@@ -65,7 +53,84 @@ Proof.
   - intros. destruct (Bool.eqb_spec x0 y0); constructor; congruence.
 Qed.
 
-(* Fixpoint expr_compatible (e1 e2 : expr) : bool := true. *)
+Definition aggregator_eqb (a1 a2 : aggregator) : bool := true.
+
+Definition aggregator_eqb_spec x y : BoolSpec (x = y) (x <> y) (aggregator_eqb x y).
+Proof.
+  destruct x, y; constructor; congruence.
+Qed.
+
+(* Right now this isn't possible because of a hiccup in Real Numbers *)
+
+Definition Bfn_eqb (f1 f2 : Bfn) : bool :=
+  match f1, f2 with
+  | fn_BAnd, fn_BAnd => true
+  | fn_BLt, fn_BLt => true
+  | fn_BLe, fn_BLe => true
+  | fn_BEq, fn_BEq => true
+  | fn_BNot, fn_BNot => true
+  | fn_BLit b1, fn_BLit b2 => Bool.eqb b1 b2
+  | _, _ => false
+  end.
+
+Lemma Bfn_eqb_spec x y : BoolSpec (x = y) (x <> y) (Bfn_eqb x y).
+Proof. 
+  destruct x, y; try (constructor; congruence); simpl;
+  try (destruct (Bool.eqb_spec b b0); constructor; congruence).
+Qed.
+
+Definition Zfn_eqb (f1 f2 : Zfn) : bool :=
+  match f1, f2 with
+  | fn_ZPlus, fn_ZPlus => true
+  | fn_ZMinus, fn_ZMinus => true
+  | fn_ZTimes, fn_ZTimes => true
+  | fn_ZDivf, fn_ZDivf => true
+  | fn_ZDivc, fn_ZDivc => true
+  | fn_ZMod, fn_ZMod => true
+  | fn_Zmax, fn_Zmax => true
+  | fn_ZRange, fn_ZRange => true
+  | fn_ZLit x, fn_ZLit y => Z.eqb x y
+  | _, _ => false
+  end.
+
+Lemma Zfn_eqb_spec x y : BoolSpec (x = y) (x <> y) (Zfn_eqb x y).
+Proof.
+  destruct x, y; try (constructor; congruence); simpl.
+  destruct (Z.eqb_spec x x0); constructor; congruence.
+Qed.
+
+Definition Rfn_eqb (f1 f2 : Rfn) : bool :=
+  match f1, f2 with
+  | fn_SMul, fn_SMul => true
+  | fn_SAdd, fn_SAdd => true
+  | fn_SDiv, fn_SDiv => true
+  | fn_SSub, fn_SSub => true
+  | fn_SLit x, fn_SLit y => true (* XXX : this is broken because it wants equality of R which is not decideable *)
+  | _, _ => false
+  end.
+
+Lemma Rfn_eqb_spec :
+  forall f1 f2,
+    BoolSpec (f1 = f2) (f1 <> f2) (Rfn_eqb f1 f2).
+Proof.
+Admitted.
+
+Definition fn_eqb (f1 f2 : fn) : bool :=
+  match f1, f2 with
+  | fn_B b1, fn_B b2 => Bfn_eqb b1 b2
+  | fn_Z z1, fn_Z z2 => Zfn_eqb z1 z2
+  | fn_R r1, fn_R r2 => Rfn_eqb r1 r2
+  | _, _ => false
+  end.
+
+Definition fn_eqb_spec x y : BoolSpec (x = y) (x <> y) (fn_eqb x y).
+Proof.
+  unfold fn_eqb.
+  destruct x, y; try (constructor; congruence).
+  - destruct (Bfn_eqb_spec b b0); constructor; congruence.
+  - destruct (Zfn_eqb_spec z z0); constructor; congruence.
+  - destruct (Rfn_eqb_spec r r0); constructor; congruence.
+Qed.
 
 Definition expr_compatible (e1 e2 : expr) : bool :=
   match e1, e2 with
