src/DependencyGenerator.v
@@ -2,9 +2,10 @@
    which will then be fed into gurobi to find an optimal layout. *)
 
 From Datalog Require Import Datalog.
-From Stdlib Require Import List.
-From Stdlib Require Import String.
-From Stdlib Require Import Bool.Bool.
+From Stdlib Require Import List String Bool Lia.
+From coqutil Require Import Datatypes.List.
+From DatalogRocq Require Import EqbSpec.
+
 Import ListNotations.
 Open Scope bool_scope.
 Open Scope string_scope.
@@ -16,10 +17,15 @@ Parameter var_eqb : var -> var -> bool.
 Parameter var_eqb_spec :  forall x0 y0 : var, BoolSpec (x0 = y0) (x0 <> y0) (var_eqb x0 y0).
 Parameter rel_eqb : rel -> rel -> bool.
 Parameter rel_eqb_spec : forall x0 y0 : rel, BoolSpec (x0 = y0) (x0 <> y0) (rel_eqb x0 y0).
+Parameter fn_eqb : fn -> fn -> bool.
+Parameter fn_eqb_spec : forall x0 y0 : fn, BoolSpec (x0 = y0) (x0 <> y0) (fn_eqb x0 y0).
+Parameter aggregator_eqb : aggregator -> aggregator -> bool.
+Parameter aggregator_eqb_spec : forall x0 y0 : aggregator, BoolSpec (x0 = y0) (x0 <> y0) (aggregator_eqb x0 y0).
 
 Definition expr := Datalog.expr var fn.
 Definition fact := Datalog.fact rel var fn.
 Definition rule := Datalog.rule rel var fn aggregator.
+Definition agg_expr := Datalog.agg_expr rel var fn aggregator.
 Definition program := list rule.
 
 Parameter expr_compatible : expr -> expr -> bool.
@@ -63,16 +69,115 @@ Definition get_const (e : expr) : option fn :=
   end.
 
 (* Eqb *)
-Fixpoint list_eqb {A : Type} (eqb : A -> A -> bool) (l1 l2 : list A) : bool :=
-  match l1, l2 with
-  | [], [] => true
-  | x :: xs, y :: ys => eqb x y && list_eqb eqb xs ys
-  | _, _ => false
+
+Fixpoint list_eqb_fuel
+  (f : expr -> expr -> nat -> bool)
+  (l1 l2 : list expr)
+  (fuel : nat) : bool :=
+  match fuel with
+  | 0 => false
+  | S fuel' =>
+      match l1, l2 with
+      | [], [] => true
+      | x1 :: xs1, x2 :: xs2 =>
+          f x1 x2 fuel' && list_eqb_fuel f xs1 xs2 fuel
+      | _, _ => false
+      end
   end.
-  
+
+Fixpoint expr_eqb_fuel (e1 e2 : expr) (fuel : nat) : bool :=
+  match fuel with
+  | 0 => false
+  | S fuel' =>
+      match e1, e2 with
+      | Datalog.var_expr v1, Datalog.var_expr v2 => var_eqb v1 v2
+      | Datalog.fun_expr f1 args1, Datalog.fun_expr f2 args2 =>
+          fn_eqb f1 f2 &&
+          list_eqb_fuel expr_eqb_fuel args1 args2 fuel'
+      | _, _ => false
+      end
+  end.
+
+Definition expr_eqb (e1 e2 : expr) : bool :=
+  expr_eqb_fuel e1 e2 (Datalog.expr_size e1 + Datalog.expr_size e2).
+
+Lemma expr_eqb_fuel_spec :
+  forall fuel e1 e2,
+    fuel >= Datalog.expr_size e1 + Datalog.expr_size e2 ->
+    BoolSpec (e1 = e2) (e1 <> e2) (expr_eqb_fuel e1 e2 fuel).
+Proof.
+ induction fuel as [|fuel IH]; intros e1 e2 Hfuel; unfold expr_eqb_fuel; simpl in *.
+ - inversion Hfuel. destruct e1; destruct e2; simpl in *; lia.
+ - destruct e1; destruct e2; simpl in *.
+   + destruct (var_eqb_spec v v0) as [Heq | Hneq].
+     * subst. constructor. reflexivity.
+     * constructor. congruence.
+   + constructor. discriminate.
+   + constructor. discriminate.
+   + destruct (fn_eqb_spec f f0) as [Hf_eq | Hf_neq]; subst.
+     *  
+Admitted.
+
+Lemma expr_eqb_spec :
+  forall e1 e2,
+    BoolSpec (e1 = e2) (e1 <> e2) (expr_eqb e1 e2).
+Proof.
+  intros. unfold expr_eqb.
+  apply expr_eqb_fuel_spec.
+  lia.
+Qed.
+
 Definition fact_eqb (f1 f2 : fact) : bool :=
   rel_eqb (fact_R f1) (fact_R f2) &&
-  list_eqb expr_compatible (fact_args f1) (fact_args f2).
+  list_eqb expr_eqb (fact_args f1) (fact_args f2).
+
+Lemma fact_eqb_spec :
+  forall f1 f2,
+    BoolSpec (f1 = f2) (f1 <> f2) (fact_eqb f1 f2).
+Proof.
+  unfold fact_eqb.
+  intros [R1 args1] [R2 args2]; simpl.
+  destruct (rel_eqb_spec R1 R2) as [HR | HR];
+  destruct (@list_eqb_spec
+            (Datalog.expr var fn)
+            expr_eqb
+            expr_eqb_spec
+            args1 args2)
+  as [Hargs | Hargs].
+  - subst. simpl. 
+Admitted.
+
+Definition agg_expr_eqb (ae1 ae2 : agg_expr) : bool :=
+  aggregator_eqb (Datalog.agg_agg ae1) (Datalog.agg_agg ae2) &&
+  var_eqb (Datalog.agg_i ae1) (Datalog.agg_i ae2) &&
+  list_eqb var_eqb (Datalog.agg_vs ae1) (Datalog.agg_vs ae2) &&
+  expr_eqb (Datalog.agg_s ae1) (Datalog.agg_s ae2) &&
+  expr_eqb (Datalog.agg_body ae1) (Datalog.agg_body ae2) &&
+  list_eqb fact_eqb (Datalog.agg_hyps ae1) (Datalog.agg_hyps ae2).
+
+Lemma agg_expr_eqb_spec :
+  forall ae1 ae2,
+    BoolSpec (ae1 = ae2) (ae1 <> ae2) (agg_expr_eqb ae1 ae2).
+Proof.
+  intros [agg1 i1 vs1 s1 body1 hyps1] [agg2 i2 vs2 s2 body2 hyps2]; simpl.
+Admitted.
+
+Definition rule_agg_eqb
+  (ra1 ra2 : option (var * agg_expr)) : bool :=
+  match ra1, ra2 with
+  | None, None => true
+  | Some (a1, ae1), Some (a2, ae2) =>
+      var_eqb a1 a2 &&
+      list_eqb fact_eqb (Datalog.agg_hyps ae1)
+                         (Datalog.agg_hyps ae2)
+  | _, _ => false
+  end.
+
+Lemma rule_agg_eqb_spec :
+  forall ra1 ra2,
+    BoolSpec (ra1 = ra2) (ra1 <> ra2) (rule_agg_eqb ra1 ra2).
+Proof.
+Admitted.
 
 Definition rule_eqb (r1 r2 : rule) : bool :=
   list_eqb fact_eqb (Datalog.rule_hyps r1) (Datalog.rule_hyps r2) &&
@@ -85,9 +190,13 @@ Definition rule_eqb (r1 r2 : rule) : bool :=
   | _, _ => false
   end.
 
+Definition rule_eqb_spec :
+  forall r1 r2,
+    BoolSpec (r1 = r2) (r1 <> r2) (rule_eqb r1 r2).
+Proof.
+Admitted.
 
 (* Pruning *)
-
 Definition prune_empty_concl_rules (p : program) : program :=
   filter (fun r => negb (list_eqb fact_eqb (Datalog.rule_concls r) [])) p.
 
@@ -229,6 +338,5 @@ Definition get_program_dependencies_by_index (p : program) : list (nat * list na
 Definition get_program_dependencies_flat (p : program) : list (nat * nat) :=
   flat_map (fun '(n, deps) => List.map (fun idx => (n, idx)) deps)
            (get_program_dependencies_by_index p).
-
 
 End DependencyGenerator.
